cclc

coq/cclc/clc_context.v
@@ -9,4 +9,331 @@ Unset Printing Implicit Defensive.
 Inductive sort : Type := U | L.
 
 Definition elem T := option (T * sort).
+Definition context T := seq (elem T).
 
+
+Notation "m :U Γ" := (Some (m, U) :: Γ) (at level 30).
+Notation "m :L Γ" := (Some (m, L) :: Γ) (at level 30).
+Notation "m :{ s } Γ" := (Some (m, s) :: Γ) (at level 30).
+Notation "_: Γ" := (None :: Γ) (at level 30).
+
+Reserved Notation "Γ1 + Γ2 => Γ" (at level 40).
+Inductive merge T : context T -> context T -> context T -> Prop :=
+| merge_nil :
+  nil + nil => nil
+| merge_left Γ1 Γ2 Γ m : 
+  Γ1 + Γ2 => Γ ->
+  m :U Γ1 + m :U Γ2 => m :U Γ
+| merge_right1 Γ1 Γ2 Γ m :
+  Γ1 + Γ2 => Γ ->
+  m :L Γ1 + _: Γ2 => m :L Γ
+| merge_right2 Γ1 Γ2 Γ m :
+  Γ1 + Γ2 => Γ ->
+  _: Γ1 + m :L Γ2 => m :L Γ
+| merge_null Γ1 Γ2 Γ :
+  Γ1 + Γ2 => Γ ->
+  _: Γ1 + _: Γ2 => _: Γ
+where "Γ1 + Γ2 => Γ" := (merge Γ1 Γ2 Γ).
+
+Reserved Notation "Γ |> s" (at level 40).
+Inductive key T : context T -> sort -> Prop :=
+| key_nil s :
+  nil |> s
+| key_u Γ m :
+  Γ |> U ->
+  m :U Γ |> U
+| key_l Γ m s :
+  Γ |> L ->
+  m :{s} Γ |> L
+| key_n Γ s :
+  Γ |> s ->
+  _: Γ |> s
+where "Γ |> s" := (key Γ s).
+
+Inductive has {T} `{Ids T} `{Subst T} :
+  context T -> var -> sort -> T -> Prop :=
+| has_O Γ A s :
+  Γ |> U ->
+  has (A :{s} Γ) 0 s A.[ren (+1)]
+| has_S Γ A B x s :    
+  has Γ x s A ->
+  has (B :U Γ) x.+1 s A.[ren (+1)]
+| has_N Γ A x s :
+  has Γ x s A ->
+  has (_: Γ) x.+1 s A.[ren (+1)].
+
+Fixpoint re T (Γ : context T) : context T :=
+  match Γ with
+  | Some (m, U) :: Γ => Some (m, U) :: re Γ
+  | _ :: Γ => None :: re Γ
+  | _ => nil
+  end.
+Notation "[ Γ ]" := (re Γ).
+
+Lemma merge_sym T (Γ1 Γ2 Γ : context T) :
+  Γ1 + Γ2 => Γ -> Γ2 + Γ1 => Γ.
+Proof.
+  elim; move=>*; eauto using merge.
+Qed.
+
+Lemma merge_pure T (Γ : context T) :
+  Γ |> U -> Γ + Γ => Γ.
+Proof.
+  move e:(U)=> s k.
+  elim: k e; move=>//=*; eauto using merge.
+Qed.
+
+Lemma merge_reL T (Γ : context T) :
+  [Γ] + Γ => Γ.
+Proof.
+  elim: Γ; eauto using merge.
+  move=> [[A[|]]|] Γ mrg//=; eauto using merge.
+Qed.
+
+Lemma merge_reR T (Γ : context T) :
+  Γ + [Γ] => Γ.
+Proof.
+  elim: Γ; eauto using merge.
+  move=> [[A[|]]|] Γ mrg//=; eauto using merge.
+Qed.
+
+Lemma merge_pure_inv T (Γ1 Γ2 Γ : context T) :
+  Γ1 + Γ2 => Γ -> Γ |> U -> Γ1 |> U /\ Γ2 |> U.
+Proof.
+  elim=>//={Γ1 Γ2 Γ}.
+  move=> Γ1 Γ2 Γ A mrg1 ih mrg2.
+    inv mrg2.
+    firstorder; eauto using key.
+  move=> Γ1 Γ2 Γ A mrg1 ih mrg2.
+    inv mrg2.
+  move=> Γ1 Γ2 Γ A mrg1 ih mrg2.
+    inv mrg2.
+  move=> Γ1 Γ2 Γ mrg1 ih mrg2.
+    inv mrg2.
+    firstorder; eauto using key.
+Qed.
+
+Lemma merge_pureL T (Γ1 Γ2 Γ : context T) :
+  Γ1 + Γ2 => Γ -> Γ1 |> U -> Γ = Γ2.
+Proof.
+  elim=>//={Γ1 Γ2 Γ}.
+  move=> Γ1 Γ2 Γ A mrg1 ih mrg2.
+    inv mrg2.
+    by rewrite ih.
+  move=> Γ1 Γ2 Γ A mrg1 ih mrg2.
+    inv mrg2.
+  move=> Γ1 Γ2 Γ A mrg1 ih mrg2.
+    inv mrg2.
+    by rewrite ih.
+  move=> Γ1 Γ2 Γ mrg1 ih mrg2.
+    inv mrg2.
+    by rewrite ih.
+Qed.
+
+Lemma merge_pure_pure T (Γ1 Γ2 Γ : context T) :
+  Γ1 + Γ2 => Γ -> Γ1 |> U -> Γ2 |> U -> Γ |> U.
+Proof.
+  elim=>//={Γ1 Γ2 Γ}.
+  move=> Γ1 Γ2 Γ A mrg ih k1 k2.
+    inv k1. inv k2.
+    by eauto using key.
+  move=> Γ1 Γ2 Γ A mrg ih k.
+    by inv k.
+  move=> Γ1 Γ2 Γ A mrg ih _ k.
+    by inv k.
+  move=> Γ1 Γ2 Γ mrg ih k1 k2.
+    inv k1. inv k2.
+    by eauto using key.
+Qed.
+
+Lemma merge_pure_eq T (Γ1 Γ2 Γ : context T) :
+  Γ1 + Γ2 => Γ -> Γ1 |> U -> Γ2 |> U -> Γ1 = Γ2.
+Proof.
+  elim=>//={Γ1 Γ2 Γ}.
+  move=> Γ1 Γ2 Γ A mrg ih k1 k2.
+    inv k1. inv k2.
+    by rewrite ih.
+  move=> Γ1 Γ2 Γ A _ _ k.
+    inv k.
+  move=> Γ1 Γ2 Γ A _ _ _ k.
+    inv k.
+  move=> Γ1 Γ2 Γ mrg ih k1 k2.
+    inv k1. inv k2.
+    by rewrite ih.
+Qed.
+
+Lemma merge_re_re T (Γ1 Γ2 Γ : context T) :
+  Γ1 + Γ2 => Γ -> [Γ1] = [Γ2] /\ [Γ1] = [Γ] /\ [Γ2] = [Γ].
+Proof.
+  elim=>//={Γ1 Γ2 Γ}.
+  move=> Γ1 Γ2 Γ A mrg[->[->_]]//.
+  move=> Γ1 Γ2 Γ A mrg[->[->_]]//.
+  move=> Γ1 Γ2 Γ A mrg[->[->_]]//.
+  move=> Γ1 Γ2 Γ mrg[->[->_]]//.
+Qed.
+
+Lemma merge_re_id T (Γ : context T) :
+  [Γ] + [Γ] => [Γ].
+Proof.
+  elim: Γ; eauto using merge.
+  move=> [[A[|]]|] Γ mrg; eauto using merge.
+Qed.
+
+Lemma re_invo T (Γ : context T) : [Γ] = [[Γ]].
+Proof.
+  elim: Γ=>//.
+  move=> [[A[|]]|] Γ//=<-//.
+Qed.
+
+Lemma pure_re T (Γ : context T) : Γ |> U -> Γ = [Γ].
+Proof.
+  elim: Γ=>//.
+  move=> [[A[|]]|] Γ ih k//=.
+  inv k. by rewrite<-ih.
+  inv k.   
+  inv k. by rewrite<-ih.
+Qed.
+
+Lemma re_pure T (Γ : context T) : [Γ] |> U.
+Proof.
+  elim: Γ; eauto using key.
+  move=> [[A[|]]|] Γ k//=; eauto using key.
+Qed.
+
+Lemma hasU_re {T} `{Ids T} `{Subst T} (Γ : context T) x A :
+  has Γ x U A -> has [Γ] x U A.
+Proof.
+  move e:(U) => s h.
+  elim: h e=>{Γ x s A}.
+  move=> Γ A s k <-//=.
+    constructor.
+    by rewrite<-pure_re.
+  move=> Γ A B x s h ih e//=; subst.
+    by constructor; eauto.
+  move=> Γ A x s h ih e//=; subst.
+    by constructor; eauto.
+Qed.
+
+Lemma hasL_re {T} `{Ids T} `{Subst T} (Γ : context T) x A :
+  ~has [Γ] x L A.
+Proof.
+  elim: Γ x A.
+  move=>//=x A h. inv h.
+  move=>[[B[|]]|] Γ ih x A //=h.
+  inv h. apply: ih; eauto.
+  inv h. apply: ih; eauto.
+  inv h. apply: ih; eauto.
+Qed.
+
+Lemma hasU_pure {T} `{Ids T} `{Subst T} (Γ : context T) x A :
+  has Γ x U A -> Γ |> U.
+Proof.
+  move e:(U)=>s h.
+  elim: h e=>{Γ x A s}.
+  move=> Γ A s ih <-; eauto using key.
+  move=> Γ A B x s h ih e; subst; eauto using key.
+  move=> Γ A x s h ih e; subst; eauto using key.
+Qed.
+
+Lemma hasL_pure {T} `{Ids T} `{Subst T} (Γ : context T) x A :
+  has Γ x L A -> ~ Γ |> U.
+Proof.
+  move e:(L)=>s h.
+  elim: h e=>{Γ x A s}.
+  move=> Γ A s k e contra; subst. inv contra.
+  move=> Γ A B x s h ih e contra. 
+    inv contra.
+    by apply: ih.
+  move=> Γ A x s h ih e contra.
+    inv contra.
+    by apply ih.
+Qed.
+
+Lemma has_inj {T} `{Ids T} `{Subst T} (Γ : context T) x s t A B :
+  has Γ x s A -> has Γ x t B -> A = B /\ s = t.
+Proof.
+  move=> h.
+  elim: h B t=>{Γ x s A}.
+  move=> Γ A s k B t h.
+    by inv h.
+  move=> Γ A B x s hA ih B0 t hB.
+    inv hB.
+    by move:(ih _ _ H6)=>[->->]//.
+  move=> Γ A x s hA ih B0 t hB.
+    inv hB.
+    by move:(ih _ _ H3)=>[->->]//.
+Qed.
+
+Lemma merge_splitL T (Γ1 Γ2 Γ : context T) :
+  Γ1 + Γ2 => Γ ->
+  forall Δ1 Δ2,
+    Δ1 + Δ2 => Γ1 ->
+    exists Δ, 
+      Δ1 + Γ2 => Δ /\ Δ + Δ2 => Γ.
+Proof.
+  elim=>{Γ1 Γ2 Γ}.
+  move=> Δ1 Δ2 mrg. 
+    inv mrg.
+    exists nil.
+    by eauto using merge.
+  move=> Γ1 Γ2 Γ A mrg ih Δ1 Δ2 mrg1.
+    inv mrg1.
+    move:(ih _ _ H2)=>[G[mrg2 mrg3]].
+    exists (A :U G).
+    by eauto using merge.
+  move=> Γ1 Γ2 Γ A mrg ih Δ1 Δ2 mrg1.
+    inv mrg1.
+    move:(ih _ _ H2)=>[G[mrg2 mrg3]].
+    exists (A :L G).
+    by eauto using merge.
+    move:(ih _ _ H2)=>[G[mrg2 mrg3]].
+    exists (_: G).
+    by eauto using merge.
+  move=> Γ1 Γ2 Γ A mrg ih Δ1 Δ2 mrg1.
+    inv mrg1.
+    move:(ih _ _ H2)=>[G[mrg2 mrg3]].
+    exists (A :L G).
+    by eauto using merge.
+  move=> Γ1 Γ2 Γ mrg ih Δ1 Δ2 mrg1.
+    inv mrg1.
+    move:(ih _ _ H2)=>[G[mrg2 mrg3]].
+    exists (_: G).
+    by eauto using merge.
+Qed.
+
+Lemma merge_splitR T (Γ1 Γ2 Γ : context T) :
+  Γ1 + Γ2 => Γ ->
+  forall Δ1 Δ2,
+    Δ1 + Δ2 => Γ1 ->
+    exists Δ,
+      Δ2 + Γ2 => Δ /\ Δ1 + Δ => Γ.
+Proof.
+  elim=>{Γ1 Γ2 Γ}.
+  move=> Δ1 Δ2 mrg. 
+    inv mrg.
+    exists nil.
+    by eauto using merge.
+  move=> Γ1 Γ2 Γ A mrg ih Δ1 Δ2 mrg1.
+    inv mrg1.
+    move:(ih _ _ H2)=>[G[mrg2 mrg3]].
+    exists (A :U G).
+    by eauto using merge.
+  move=> Γ1 Γ2 Γ A mrg ih Δ1 Δ2 mrg1.
+    inv mrg1.
+    move:(ih _ _ H2)=>[G[mrg2 mrg3]].
+    exists (_: G).
+    by eauto using merge.
+    move:(ih _ _ H2)=>[G[mrg2 mrg3]].
+    exists (A :L G).
+    by eauto using merge.
+  move=> Γ1 Γ2 Γ A mrg ih Δ1 Δ2 mrg1.
+    inv mrg1.
+    move:(ih _ _ H2)=>[G[mrg2 mrg3]].
+    exists (A :L G).
+    by eauto using merge.
+  move=> Γ1 Γ2 Γ mrg ih Δ1 Δ2 mrg1.
+    inv mrg1.
+    move:(ih _ _ H2)=>[G[mrg2 mrg3]].
+    exists (_: G).
+    by eauto using merge.
+Qed.
